ROOT
@@ -1341,6 +1341,7 @@ session RRA_Factor_Structural_Bootstrap = HOL +
     Finite_Presented_Collections
     Factor_Least_Collections
     Factor_Least_Witness_Registrations
+    Factor_Narrowed_Sockets
     Factor_Varied_Constructions
     Factor_Reader_Witness_Registrations
     Finite_Presented_Coordinates
